Syncing the soundness proof with paper

state/MST.Soundness.fst
@@ -29,17 +29,17 @@ let heap_rel (h1:heap) (h2:heap) =
 
 let stable (pred: heap -> Type0) = stable pred heap_rel
 
-type stable_pred =
+type heap_predicate_stable =
   pred:(heap -> Type0){forall h0 h1. pred h0 /\ h0 `heap_rel` h1 ==> pred h1}
 
 let state_wp a = (a -> heap -> Type0) -> (heap -> Type0)
 
-let state_wp_return (x:'a) : state_wp 'a = fun p s0 -> p x s0
+let state_wp_return (x:'a) : state_wp 'a = fun p h0 -> p x h0
 let state_wp_bind (m:state_wp 'a) (k:'a -> state_wp 'b) : state_wp 'b =
-  fun p s0 -> m (fun r s1 -> k r p s1) s0
+  fun p h0 -> m (fun r h1 -> k r p h1) h0
 
 let state_wp_stronger (wp1 wp2:state_wp 'a) : Type0 =
-  forall p s0. wp2 p s0 ==> wp1 p s0
+  forall p h0. wp2 p h0 ==> wp1 p h0
 
 noeq
 type mst_repr (a:Type) =
@@ -47,8 +47,8 @@ type mst_repr (a:Type) =
 | Read : #b:Type0 -> #rel: preorder b -> r: mref b rel -> cont:(b -> mst_repr a) -> mst_repr a
 | Write : #b:Type0 -> #rel: preorder b -> r: mref b rel -> v:b -> cont:mst_repr a -> mst_repr a
 | Alloc : #b:Type0 -> #rel: preorder b -> init: b -> cont:(mref b rel -> mst_repr a) -> mst_repr a
-| Witness : pred:stable_pred -> (unit -> mst_repr a) -> mst_repr a
-| Recall : pred:stable_pred -> (unit -> mst_repr a) -> mst_repr a
+| Witness : pred:heap_predicate_stable -> (unit -> mst_repr a) -> mst_repr a
+| Recall : pred:heap_predicate_stable -> (unit -> mst_repr a) -> mst_repr a
 
 unfold
 let read_wp (#a:Type) (#rel:preorder a) (r:mref a rel) : state_wp a =
@@ -101,7 +101,7 @@ let rec theta (witnessed:(heap -> Type0) -> Type0) (m:mst_repr 'a) : state_wp 'a
 
 module S = FStar.TSet
 
-let rec witnessed_before #a (preds:S.set stable_pred) (m:mst_repr a) : Tot Type0 (decreases m) =
+let rec witnessed_before #a (preds:S.set heap_predicate_stable) (m:mst_repr a) : Tot Type0 (decreases m) =
   match m with
   | Return _ -> True
   | Read r k -> forall v . preds `witnessed_before` (k v)
@@ -111,69 +111,69 @@ let rec witnessed_before #a (preds:S.set stable_pred) (m:mst_repr a) : Tot Type0
   | Recall pred k -> pred `S.mem` preds /\ preds `witnessed_before` (k ())
 
 type heap_w_preds =
-  sp:(heap * S.set stable_pred){forall (pred:stable_pred). pred `S.mem` (snd sp) ==> pred (fst sp)}
+  hp:(heap * S.set heap_predicate_stable){forall (pred:heap_predicate_stable). pred `S.mem` (snd hp) ==> pred (fst hp)}
   
 val witnessed_trivial : (heap -> Type0) -> Type0
 let witnessed_trivial pred = True // trivial instance of witnessed tokens
 
 let rec run_mst_with_preds #a 
-  (m:mst_repr a) 
-  (wp:(state_wp a){theta witnessed_trivial m `state_wp_stronger` wp}) 
+  (wp:state_wp a) 
+  (m:mst_repr a{theta witnessed_trivial m `state_wp_stronger` wp}) 
   (post:(a -> heap -> Type0)) 
-  (s0:heap_w_preds{wp post (fst s0) /\ (snd s0) `witnessed_before` m}) 
+  (h0:heap_w_preds{wp post (fst h0) /\ (snd h0) `witnessed_before` m}) 
 : Tot (r:(a * heap_w_preds){post (fst r) (fst (snd r))}) 
 =
   match m with
-  | Return x -> (x, s0)
+  | Return v -> (v, h0)
   | Read #_ #b #rel r k -> 
-      lemma_sel_equals_sel_tot_for_contained_refs (fst s0) r;
-      run_mst_with_preds (k (sel_tot (fst s0) r)) (theta witnessed_trivial (k (sel_tot (fst s0) r))) post s0
+      lemma_sel_equals_sel_tot_for_contained_refs (fst h0) r;
+      run_mst_with_preds (theta witnessed_trivial (k (sel_tot (fst h0) r))) (k (sel_tot (fst h0) r)) post h0
   | Write #_ #b #rel r v k -> 
-      lemma_upd_equals_upd_tot_for_contained_refs (fst s0) r v;
-      introduce forall (a':Type0) (rel':preorder a') (r':mref a' rel'). fst s0 `contains` r' ==> 
-        (upd (fst s0) r v `contains` r' /\ rel' (sel (fst s0) r') (sel (upd (fst s0) r v) r')) with
+      lemma_upd_equals_upd_tot_for_contained_refs (fst h0) r v;
+      introduce forall (a':Type0) (rel':preorder a') (r':mref a' rel'). fst h0 `contains` r' ==> 
+        (upd (fst h0) r v `contains` r' /\ rel' (sel (fst h0) r') (sel (upd (fst h0) r v) r')) with
       begin
-        introduce fst s0 `contains` r' /\ addr_of r = addr_of r' ==> 
-          (upd (fst s0) r v `contains` r' /\ rel' (sel (fst s0) r') (sel (upd (fst s0) r v) r')) with _.
+        introduce fst h0 `contains` r' /\ addr_of r = addr_of r' ==> 
+          (upd (fst h0) r v `contains` r' /\ rel' (sel (fst h0) r') (sel (upd (fst h0) r v) r')) with _.
         begin
-          lemma_eq_addrs_eq_all r r' (fst s0)
+          lemma_eq_addrs_eq_all r r' (fst h0)
         end
       end;
-      run_mst_with_preds k (theta witnessed_trivial k) post (upd_tot (fst s0) r v, snd s0)
+      run_mst_with_preds (theta witnessed_trivial k) k post (upd_tot (fst h0) r v, snd h0)
   | Alloc #_ #b #rel init k -> 
-      let (r,h) = alloc rel (fst s0) init false in
+      let (r,h) = alloc rel (fst h0) init false in
       lemma_upd_equals_upd_tot_for_contained_refs h r init;
-      assert (fst s0 `heap_rel` upd (fst s0) r init);
-      lemma_alloc rel (fst s0) init false;
-      lemma_next_addr_alloc rel (fst s0) init false;
-      run_mst_with_preds (k r) (theta witnessed_trivial (k r)) post (h,snd s0)
+      assert (fst h0 `heap_rel` upd (fst h0) r init);
+      lemma_alloc rel (fst h0) init false;
+      lemma_next_addr_alloc rel (fst h0) init false;
+      run_mst_with_preds (theta witnessed_trivial (k r)) (k r) post (h,snd h0)
   | Witness pred k -> 
-    let lp = S.union (snd s0) (S.singleton pred) in
-    run_mst_with_preds (k ()) (theta witnessed_trivial (k ())) post (fst s0, lp)
+      let hp = S.union (snd h0) (S.singleton pred) in
+      run_mst_with_preds (theta witnessed_trivial (k ())) (k ()) post (fst h0, hp)
   | Recall pred k -> 
-    run_mst_with_preds (k ()) (theta witnessed_trivial (k ())) post s0
+      run_mst_with_preds (theta witnessed_trivial (k ())) (k ()) post h0
 
 let run_mst #a 
-  (m:mst_repr a{S.empty `witnessed_before` m}) 
-  (wp:(state_wp a){theta witnessed_trivial m `state_wp_stronger` wp}) 
+  (wp:state_wp a) 
+  (m:mst_repr a{theta witnessed_trivial m `state_wp_stronger` wp /\ S.empty `witnessed_before` m}) 
   (post:(a -> heap -> Type0)) 
-  (s0:heap{wp post s0}) 
-: Tot (r:(a * heap){post (fst r) (snd r)}) 
+  (h0:heap{wp post h0}) 
+: Tot (vh:(a * heap){post (fst vh) (snd vh)}) 
 =
-  let (r, s1p) = run_mst_with_preds m wp post (s0, S.empty) in
-  (r, fst s1p)
+  let (v, h1) = run_mst_with_preds wp m post (h0, S.empty) in
+  (v, fst h1)
   
-let soundness_with_preds #a (m:mst_repr a) (wp:state_wp a) (preds:S.set stable_pred) 
+let soundness_with_preds #a (m:mst_repr a) (wp:state_wp a) (preds:S.set heap_predicate_stable) 
 : Lemma
     (requires ((forall witnessed. theta witnessed m `state_wp_stronger` wp) /\ preds `witnessed_before` m))
-    (ensures  (forall post s0. wp post s0 /\ (forall (pred:stable_pred). pred `S.mem` preds ==> pred s0) ==> 
-                            (let (r,s1p) = run_mst_with_preds m wp post (s0, preds) in post r (fst s1p)))) 
+    (ensures  (forall post h0. wp post h0 /\ (forall (pred:heap_predicate_stable). pred `S.mem` preds ==> pred h0) ==> 
+                            (let (r,h1p) = run_mst_with_preds wp m post (h0, preds) in post r (fst h1p)))) 
 =
   () 
 
 let soundness_whole_program #a (m:mst_repr a) (wp:state_wp a) 
 : Lemma 
     (requires ((forall witnessed. theta witnessed m `state_wp_stronger` wp) /\ S.empty `witnessed_before` m)) 
-    (ensures  (forall post s0. wp post s0 ==> (let (r,s1) = run_mst m wp post s0 in post r s1))) 
+    (ensures  (forall post h0. wp post h0 ==> (let (r,h1) = run_mst wp m post h0 in post r h1))) 
 =
   ()
